src/basic/FStarC.Options.fsti
@@ -219,10 +219,12 @@ val custard_max_specializations : unit    -> ML int
 val custard_norm_budget         : unit    -> ML int
 val custard_monomorphize_types  : unit    -> ML bool
 val custard_backend             : unit    -> ML string
+val custard_backend_krml        : unit    -> ML bool
 val custard_split               : unit    -> ML bool
 val custard_unit                : unit    -> ML (option string)
 val custard_links               : unit    -> ML (list string)
 val custard_extern_types        : unit    -> ML (list string)
+val custard_krml_models         : unit    -> ML (list string)
 val custard_dump_cui            : unit    -> ML bool
 
 val profile_group_by_decl       : unit    -> ML bool
